examples/low-level/merkletree/MerkleTree.High.fst
@@ -1,6 +1,7 @@
 module MerkleTree.High
 
 open FStar.All
+open FStar.Ghost
 open FStar.Mul
 open FStar.Seq
 open FStar.Integers
@@ -8,341 +9,247 @@ open FStar.Integers
 module List = FStar.List.Tot
 module S = FStar.Seq
 
+module U32 = FStar.UInt32
 module U8 = FStar.UInt8
+type uint32_t = U32.t
 type uint8_t = U8.t
 
-noextract val hash_size: nat
-noextract let hash_size = 32
+val hash_size: uint32_t
+let hash_size = 32ul
 
-type bytes = S.seq UInt8.t
-type hash = b:bytes{S.length b = hash_size}
+let hash = b:S.seq uint8_t{S.length b = U32.v hash_size}
 let hash_seq = S.seq hash
 
 assume val hash_from_hashes: hash -> hash -> Tot hash
 
 /// About FStar.Seq.Base.seq
 
-val lemma_split_append:
-  #a:Type -> s1:S.seq a -> s2:S.seq a ->
-  Lemma (S.split (S.append s1 s2) (S.length s1) == (s1, s2))
-let lemma_split_append #a s1 s2 =
-  S.lemma_eq_elim (fst (S.split (S.append s1 s2) (S.length s1))) s1;
-  S.lemma_eq_elim (snd (S.split (S.append s1 s2) (S.length s1))) s2
+// val lemma_split_append:
+//   #a:Type -> s1:S.seq a -> s2:S.seq a ->
+//   Lemma (S.split (S.append s1 s2) (S.length s1) == (s1, s2))
+// let lemma_split_append #a s1 s2 =
+//   S.lemma_eq_elim (fst (S.split (S.append s1 s2) (S.length s1))) s1;
+//   S.lemma_eq_elim (snd (S.split (S.append s1 s2) (S.length s1))) s2
 
-val seq_create_one_cons:
-  #a:eqtype -> ia:a -> 
-  Lemma (S.create 1 ia = S.cons ia S.empty)
-	[SMTPat (S.create 1 ia); SMTPat (S.cons ia S.empty)]
-let seq_create_one_cons #a ia =
-  S.lemma_eq_elim (S.create 1 ia) (S.cons ia S.empty)
+// val seq_create_one_cons:
+//   #a:eqtype -> ia:a -> 
+//   Lemma (S.create 1 ia = S.cons ia S.empty)
+// 	[SMTPat (S.create 1 ia); SMTPat (S.cons ia S.empty)]
+// let seq_create_one_cons #a ia =
+//   S.lemma_eq_elim (S.create 1 ia) (S.cons ia S.empty)
 
 /// Power of two
 
-val is_pow2: nat -> Tot bool
-let rec is_pow2 n =
-  if n = 0 then false
-  else if n = 1 then true
-  else (n % 2 = 0 && is_pow2 (n / 2))
+// val is_pow2: nat -> Tot bool
+// let rec is_pow2 n =
+//   if n = 0 then false
+//   else if n = 1 then true
+//   else (n % 2 = 0 && is_pow2 (n / 2))
 
-val pow2_is_pow2:
-  n:nat ->
-  Lemma (is_pow2 (pow2 n))
-	[SMTPat (is_pow2 (pow2 n))]
-let rec pow2_is_pow2 n =
-  if n = 0 then ()
-  else pow2_is_pow2 (n - 1)
+// val pow2_is_pow2:
+//   n:nat ->
+//   Lemma (is_pow2 (pow2 n))
+// 	[SMTPat (is_pow2 (pow2 n))]
+// let rec pow2_is_pow2 n =
+//   if n = 0 then ()
+//   else pow2_is_pow2 (n - 1)
 
-val pow2_lt_le:
-  n:nat -> p:nat{p > 0} ->
-  Lemma (requires (is_pow2 n && n < pow2 p))
-	(ensures (n <= pow2 (p - 1)))
-let rec pow2_lt_le n p =
-  if n = 1 then ()
-  else pow2_lt_le (n / 2) (p - 1)
+// val pow2_lt_le:
+//   n:nat -> p:nat{p > 0} ->
+//   Lemma (requires (is_pow2 n && n < pow2 p))
+// 	(ensures (n <= pow2 (p - 1)))
+// let rec pow2_lt_le n p =
+//   if n = 1 then ()
+//   else pow2_lt_le (n / 2) (p - 1)
 
-val pow2_floor: 
-  n:nat{n > 0} -> GTot (p:nat{pow2 p <= n && n < pow2 (p + 1)})
-let rec pow2_floor n =
-  if n = 1 then 0 else 1 + pow2_floor (n / 2)
+// val pow2_floor: 
+//   n:nat{n > 0} -> GTot (p:nat{pow2 p <= n && n < pow2 (p + 1)})
+// let rec pow2_floor n =
+//   if n = 1 then 0 else 1 + pow2_floor (n / 2)
 
-val pow2_ceil:
-  n:nat{n > 0} -> 
-  GTot (p:nat{
-    if n = 1 then p = 0
-    else (p > 0 && pow2 (p - 1) < n && n <= pow2 p)})
-let rec pow2_ceil n =
-  if n = 1 then 0
-  else if n % 2 = 0 then 1 + pow2_ceil (n / 2)
-  else 1 + pow2_ceil ((n + 1) / 2)
+// val pow2_ceil:
+//   n:nat{n > 0} -> 
+//   GTot (p:nat{
+//     if n = 1 then p = 0
+//     else (p > 0 && pow2 (p - 1) < n && n <= pow2 p)})
+// let rec pow2_ceil n =
+//   if n = 1 then 0
+//   else if n % 2 = 0 then 1 + pow2_ceil (n / 2)
+//   else 1 + pow2_ceil ((n + 1) / 2)
 
-val pow2_floor_pow2:
-  p:nat -> 
-  Lemma (pow2_floor (pow2 p) = p)
-	[SMTPat (pow2_floor (pow2 p))]
-let rec pow2_floor_pow2 p =
-  if p = 0 then ()
-  else pow2_floor_pow2 (p - 1)
+// val pow2_floor_pow2:
+//   p:nat -> 
+//   Lemma (pow2_floor (pow2 p) = p)
+// 	[SMTPat (pow2_floor (pow2 p))]
+// let rec pow2_floor_pow2 p =
+//   if p = 0 then ()
+//   else pow2_floor_pow2 (p - 1)
 
-val pow2_ceil_pow2:
-  p:nat -> 
-  Lemma (pow2_ceil (pow2 p) = p)
-	[SMTPat (pow2_ceil (pow2 p))]
-let rec pow2_ceil_pow2 p =
-  if p = 0 then ()
-  else (assert (pow2 p / 2 = pow2 (p - 1));
-       pow2_ceil_pow2 (p - 1))
+// val pow2_ceil_pow2:
+//   p:nat -> 
+//   Lemma (pow2_ceil (pow2 p) = p)
+// 	[SMTPat (pow2_ceil (pow2 p))]
+// let rec pow2_ceil_pow2 p =
+//   if p = 0 then ()
+//   else (assert (pow2 p / 2 = pow2 (p - 1));
+//        pow2_ceil_pow2 (p - 1))
 
-val pow2_floor_is_pow2:
-  n:nat ->
-  Lemma (requires (is_pow2 n))
-	(ensures (n = pow2 (pow2_floor n)))
-	[SMTPat (is_pow2 n)]
-let rec pow2_floor_is_pow2 n =
-  if n = 1 then ()
-  else pow2_floor_is_pow2 (n / 2)
+// val pow2_floor_is_pow2:
+//   n:nat ->
+//   Lemma (requires (is_pow2 n))
+// 	(ensures (n = pow2 (pow2_floor n)))
+// 	[SMTPat (is_pow2 n)]
+// let rec pow2_floor_is_pow2 n =
+//   if n = 1 then ()
+//   else pow2_floor_is_pow2 (n / 2)
 
-val pow2_ceil_is_pow2:
-  n:nat ->
-  Lemma (requires (is_pow2 n))
-	(ensures (n = pow2 (pow2_ceil n)))
-	[SMTPat (is_pow2 n)]
-let rec pow2_ceil_is_pow2 n =
-  if n = 1 then ()
-  else pow2_ceil_is_pow2 (n / 2)
+// val pow2_ceil_is_pow2:
+//   n:nat ->
+//   Lemma (requires (is_pow2 n))
+// 	(ensures (n = pow2 (pow2_ceil n)))
+// 	[SMTPat (is_pow2 n)]
+// let rec pow2_ceil_is_pow2 n =
+//   if n = 1 then ()
+//   else pow2_ceil_is_pow2 (n / 2)
 
-val pow2_interval_unique:
-  n:nat -> p1:nat -> p2:nat ->
-  Lemma (requires (pow2 p1 <= n && n < pow2 (p1 + 1) &&
-		  pow2 p2 <= n && n < pow2 (p2 + 1)))
-	(ensures (p1 = p2))
-let pow2_interval_unique n p1 p2 =
-  if p1 > p2 
-  then Math.Lemmas.pow2_le_compat (p1 - 1) p2
-  else if p1 < p2
-  then Math.Lemmas.pow2_le_compat (p2 - 1) p1
-  else ()
+// val pow2_interval_unique:
+//   n:nat -> p1:nat -> p2:nat ->
+//   Lemma (requires (pow2 p1 <= n && n < pow2 (p1 + 1) &&
+// 		  pow2 p2 <= n && n < pow2 (p2 + 1)))
+// 	(ensures (p1 = p2))
+// let pow2_interval_unique n p1 p2 =
+//   if p1 > p2 
+//   then Math.Lemmas.pow2_le_compat (p1 - 1) p2
+//   else if p1 < p2
+//   then Math.Lemmas.pow2_le_compat (p2 - 1) p1
+//   else ()
 
-val pow2_floor_inv:
-  p:nat -> n:nat{pow2 p <= n && n < pow2 (p + 1)} ->
-  Lemma (pow2_floor n = p)
-let pow2_floor_inv p n =
-  pow2_interval_unique n (pow2_floor n) p
+// val pow2_floor_inv:
+//   p:nat -> n:nat{pow2 p <= n && n < pow2 (p + 1)} ->
+//   Lemma (pow2_floor n = p)
+// let pow2_floor_inv p n =
+//   pow2_interval_unique n (pow2_floor n) p
 
-val pow2_floor_pow2_less:
-  p:nat -> n:nat{n < pow2 p} ->
-  Lemma (pow2_floor (pow2 p + n) = p)
-let pow2_floor_pow2_less p n =
-  pow2_floor_inv p (pow2 p + n)
+// val pow2_floor_pow2_less:
+//   p:nat -> n:nat{n < pow2 p} ->
+//   Lemma (pow2_floor (pow2 p + n) = p)
+// let pow2_floor_pow2_less p n =
+//   pow2_floor_inv p (pow2 p + n)
 
-val pow2_floor_pow2_pow2:
-  p:nat -> q:nat{p > q} ->
-  Lemma (pow2_floor (pow2 p + pow2 q) = p)
-let pow2_floor_pow2_pow2 p q =
-  Math.Lemmas.pow2_lt_compat p q;
-  pow2_floor_pow2_less p (pow2 q)
+// val pow2_floor_pow2_pow2:
+//   p:nat -> q:nat{p > q} ->
+//   Lemma (pow2_floor (pow2 p + pow2 q) = p)
+// let pow2_floor_pow2_pow2 p q =
+//   Math.Lemmas.pow2_lt_compat p q;
+//   pow2_floor_pow2_less p (pow2 q)
 
-val pow2_lt_compat_inv:
-  p:nat -> q:nat ->
-  Lemma (requires (pow2 p < pow2 q))
-	(ensures (p < q))
-let rec pow2_lt_compat_inv p q =
-  if q <= p then Math.Lemmas.pow2_le_compat p q
-  else ()
+// val pow2_lt_compat_inv:
+//   p:nat -> q:nat ->
+//   Lemma (requires (pow2 p < pow2 q))
+// 	(ensures (p < q))
+// let rec pow2_lt_compat_inv p q =
+//   if q <= p then Math.Lemmas.pow2_le_compat p q
+//   else ()
 
-val pow2_le_compat_inv:
-  p:nat -> q:nat ->
-  Lemma (requires (pow2 p <= pow2 q))
-	(ensures (p <= q))
-let rec pow2_le_compat_inv p q =
-  if q < p then Math.Lemmas.pow2_lt_compat p q
-  else ()
+// val pow2_le_compat_inv:
+//   p:nat -> q:nat ->
+//   Lemma (requires (pow2 p <= pow2 q))
+// 	(ensures (p <= q))
+// let rec pow2_le_compat_inv p q =
+//   if q < p then Math.Lemmas.pow2_lt_compat p q
+//   else ()
 
-val not_pow2_floor_ceil:
-  n:nat{n > 0 && not (is_pow2 n)} ->
-  Lemma (pow2_floor n + 1 = pow2_ceil n)
-let not_pow2_floor_ceil n =
-  let fl = pow2_floor n in
-  let cl = pow2_ceil n in
-  pow2_le_compat_inv fl cl;
-  pow2_lt_compat_inv (cl - 1) (fl + 1)
-
-val num_of_ones: nelts:nat -> GTot nat
-let rec num_of_ones nelts =
-  if nelts = 0 then 0
-  else 1 + num_of_ones (nelts - pow2 (pow2_floor nelts))
+// val not_pow2_floor_ceil:
+//   n:nat{n > 0 && not (is_pow2 n)} ->
+//   Lemma (pow2_floor n + 1 = pow2_ceil n)
+// let not_pow2_floor_ceil n =
+//   let fl = pow2_floor n in
+//   let cl = pow2_ceil n in
+//   pow2_le_compat_inv fl cl;
+//   pow2_lt_compat_inv (cl - 1) (fl + 1)
 
 /// Invariants between internal roots and values
 
-type hash_seq_pow2 = hs:hash_seq{is_pow2 (S.length hs)}
+// type hash_seq_pow2 = hs:hash_seq{is_pow2 (S.length hs)}
 
-val merkle_root_of_pow2:
-  hs:hash_seq_pow2 -> GTot hash (decreases (S.length hs))
-let rec merkle_root_of_pow2 hs =
-  if S.length hs = 1 then S.index hs 0
-  else
-    let lhs, rhs = S.split hs (S.length hs / 2) in
-    let lrt = merkle_root_of_pow2 lhs in
-    let rrt = merkle_root_of_pow2 rhs in
-    hash_from_hashes lrt rrt
+// val merkle_root_of_pow2:
+//   hs:hash_seq_pow2 -> GTot hash (decreases (S.length hs))
+// let rec merkle_root_of_pow2 hs =
+//   if S.length hs = 1 then S.index hs 0
+//   else
+//     let lhs, rhs = S.split hs (S.length hs / 2) in
+//     let lrt = merkle_root_of_pow2 lhs in
+//     let rrt = merkle_root_of_pow2 rhs in
+//     hash_from_hashes lrt rrt
 
-val merkle_root_of_pow2_inv:
-  hs1:hash_seq_pow2{S.length hs1 > 0} -> 
-  hs2:hash_seq_pow2{S.length hs2 = S.length hs1} ->
-  Lemma (merkle_root_of_pow2 (S.append hs1 hs2) =
-	hash_from_hashes (merkle_root_of_pow2 hs1)
-			 (merkle_root_of_pow2 hs2))
-	[SMTPat (merkle_root_of_pow2 (S.append hs1 hs2))]
-let merkle_root_of_pow2_inv hs1 hs2 =
-  assert (S.length (S.append hs1 hs2) / 2 = S.length hs1);
-  lemma_split_append hs1 hs2
-
-val iroots_of_hashes:
-  hs:hash_seq -> 
-  GTot (iroots:hash_seq{S.length iroots = num_of_ones (S.length hs)})
-       (decreases (S.length hs))
-let rec iroots_of_hashes hs =
-  if S.length hs = 0 then hs
-  else
-    let n_floor = pow2 (pow2_floor (S.length hs)) in
-    let hs0, hs1 = S.split hs n_floor in
-    S.cons (merkle_root_of_pow2 hs0) (iroots_of_hashes hs1)
-
-val iroots_of_hashes_pow2_same:
-  hs1:hash_seq_pow2 ->
-  hs2:hash_seq{S.length hs2 = S.length hs1} ->
-  Lemma (iroots_of_hashes (S.append hs1 hs2) =
-	S.create 1 (hash_from_hashes 
-	  (S.index (iroots_of_hashes hs1) 0)
-	  (S.index (iroots_of_hashes hs2) 0)))
-let iroots_of_hashes_pow2_same hs1 hs2 =
-  S.lemma_eq_elim (S.cons (merkle_root_of_pow2 (S.append hs1 hs2)) S.empty)
-  		  (S.create 1 (merkle_root_of_pow2 (S.append hs1 hs2)));
-  assert (S.index (iroots_of_hashes hs1) 0 = merkle_root_of_pow2 hs1);
-  assert (S.index (iroots_of_hashes hs2) 0 = merkle_root_of_pow2 hs2)
-
-val iroots_of_hashes_pow2_diff:
-  hs1:hash_seq_pow2 ->
-  hs2:hash_seq{S.length hs1 > S.length hs2} ->
-  Lemma (iroots_of_hashes (S.append hs1 hs2) =
-	S.append (iroots_of_hashes hs1) (iroots_of_hashes hs2))
-let iroots_of_hashes_pow2_diff hs1 hs2 =
-  pow2_floor_pow2_less (pow2_floor (S.length hs1)) (S.length hs2);
-  lemma_split_append hs1 hs2;
-  S.lemma_eq_elim
-    (S.cons (merkle_root_of_pow2 hs1) (iroots_of_hashes hs2))
-    (S.append (S.cons (merkle_root_of_pow2 hs1) S.empty)
-	      (iroots_of_hashes hs2))
+// val merkle_root_of_pow2_inv:
+//   hs1:hash_seq_pow2{S.length hs1 > 0} -> 
+//   hs2:hash_seq_pow2{S.length hs2 = S.length hs1} ->
+//   Lemma (merkle_root_of_pow2 (S.append hs1 hs2) =
+// 	hash_from_hashes (merkle_root_of_pow2 hs1)
+// 			 (merkle_root_of_pow2 hs2))
+// 	[SMTPat (merkle_root_of_pow2 (S.append hs1 hs2))]
+// let merkle_root_of_pow2_inv hs1 hs2 =
+//   assert (S.length (S.append hs1 hs2) / 2 = S.length hs1);
+//   lemma_split_append hs1 hs2
 
 /// High-level Merkle tree data structure
 
 noeq type merkle_tree =
-| MT: values:hash_seq ->
-      iroots:hash_seq{iroots = iroots_of_hashes values} ->
+| MT: sz:nat ->
+      values:hash_seq{S.length values < pow2 sz} ->
+      iroots:hash_seq{S.length iroots = sz} ->
       merkle_tree
 
 /// Creating a merkle tree instance
 
-val create_merkle_tree: unit -> merkle_tree
-let create_merkle_tree _ =
-  MT S.empty S.empty
+val hash_default: hash
+let hash_default = S.create (U32.v hash_size) 0uy
+
+val create_merkle_tree: nat -> Tot merkle_tree
+let create_merkle_tree sz =
+  MT sz S.empty (S.create sz hash_default)
 
 /// Insertion
 
-val insert_values: hash_seq -> hash -> GTot hash_seq
-let insert_values vs nv = S.snoc vs nv
-
-val merge_iroots:
-  vs1:hash_seq_pow2 -> 
-  irs1:hash_seq{iroots_of_hashes vs1 = irs1} ->
-  vs2:hash_seq{S.length vs1 >= S.length vs2} ->
-  irs2:hash_seq{iroots_of_hashes vs2 = irs2} ->
-  GTot (mirs:hash_seq{iroots_of_hashes (S.append vs1 vs2) = mirs})
-let merge_iroots vs1 irs1 vs2 irs2 =
-  if S.length vs1 = S.length vs2
-  then (iroots_of_hashes_pow2_same vs1 vs2; 
-       S.create 1 (hash_from_hashes (S.index irs1 0) (S.index irs2 0)))
-  else (iroots_of_hashes_pow2_diff vs1 vs2; 
-       S.append irs1 irs2)
-
-val iroots_of_hashes_head:
-  vs:hash_seq{S.length vs > 0} ->
-  irs:hash_seq{iroots_of_hashes vs = irs} ->
-  Lemma (merkle_root_of_pow2 (S.slice vs 0 (pow2 (pow2_floor (S.length vs)))) = 
-	S.head irs)
-let iroots_of_hashes_head vs irs =
-  let n_floor = pow2 (pow2_floor (S.length vs)) in
-  let hs0, hs1 = S.split vs n_floor in 
-  S.head_cons (merkle_root_of_pow2 (S.slice vs 0 n_floor)) (iroots_of_hashes hs1)
-
-val iroots_of_hashes_tail:
-  vs:hash_seq{S.length vs > 0} ->
-  irs:hash_seq{iroots_of_hashes vs = irs} ->
-  Lemma (iroots_of_hashes (S.slice vs (pow2 (pow2_floor (S.length vs))) (S.length vs)) =
-	S.tail irs)
-#set-options "--z3rlimit 10"
-let iroots_of_hashes_tail vs irs =
-  let n_floor = pow2 (pow2_floor (S.length vs)) in
-  S.lemma_tl (merkle_root_of_pow2 (S.slice vs 0 n_floor))
-	     (iroots_of_hashes (S.slice vs n_floor (S.length vs)))
-
-val iroots_of_head:
-  vs:hash_seq{S.length vs > 0} ->
-  Lemma (iroots_of_hashes (S.slice vs 0 (pow2 (pow2_floor (S.length vs)))) =
-	S.create 1 (S.head (iroots_of_hashes vs)))
-let iroots_of_head vs =
-  let n_floor = pow2 (pow2_floor (S.length vs)) in
-  assert (S.head (iroots_of_hashes vs) = merkle_root_of_pow2 (S.slice vs 0 n_floor))
-
-val iroots_of_tail:
-  vs:hash_seq{S.length vs > 0} ->
-  Lemma (iroots_of_hashes (S.slice vs (pow2 (pow2_floor (S.length vs))) (S.length vs)) =
-	S.tail (iroots_of_hashes vs))
-let iroots_of_tail vs =
-  let n_floor = pow2 (pow2_floor (S.length vs)) in
-  S.lemma_tl (merkle_root_of_pow2 (S.slice vs 0 n_floor))
-	     (iroots_of_hashes (S.slice vs n_floor (S.length vs)))
+val insert_values: 
+  sz:nat -> hs:hash_seq{S.length hs < pow2 sz - 1} -> hash -> 
+  Tot (ihs:hash_seq{S.length ihs < pow2 sz})
+let insert_values sz vs nv = S.snoc vs nv
 
 val insert_iroots:
-  vs:hash_seq ->
-  irs:hash_seq{iroots_of_hashes vs = irs} ->
-  nv:hash ->
-  GTot (iirs:hash_seq{iroots_of_hashes (insert_values vs nv) = iirs})
-       (decreases (S.length irs))
-#set-options "--z3rlimit 80"
-let rec insert_iroots vs irs nv =
-  if S.length vs = 0
-  then S.create 1 nv
-  else if is_pow2 (S.length vs)
-  then merge_iroots vs irs (S.create 1 nv) (S.create 1 nv)
-  else
-    (let vs0, vs1 = S.split vs (pow2 (pow2_floor (S.length vs))) in
-    lemma_split vs (pow2 (pow2_floor (S.length vs)));
-    iroots_of_head vs;
-    iroots_of_tail vs;
-    append_assoc vs0 vs1 (S.create 1 nv);
-    merge_iroots vs0 (S.create 1 (S.head irs)) (insert_values vs1 nv) 
-		 (insert_iroots vs1 (S.tail irs) nv))
+  irs:hash_seq ->
+  cpos:nat{cpos < S.length irs} ->
+  irps:nat{irps < pow2 (S.length irs - cpos) - 1} ->
+  acc:hash ->
+  Tot (iirs:hash_seq{S.length iirs = S.length irs})
+      (decreases (S.length irs - cpos))
+let rec insert_iroots irs cpos irps acc =
+  if irps % 2 = 0
+  then S.upd irs cpos acc
+  else (let nacc = hash_from_hashes (S.index irs cpos) acc in
+       insert_iroots irs (cpos + 1) (irps / 2) nacc)
 
 val insert: 
-  mt:merkle_tree -> e:hash -> 
-  GTot (imt:merkle_tree{
-    MT?.values imt = insert_values (MT?.values mt) e &&
-    MT?.iroots imt = insert_iroots (MT?.values mt) (MT?.iroots mt) e})
+  mt:merkle_tree{S.length (MT?.values mt) < pow2 (MT?.sz mt) - 1} ->
+  e:hash -> Tot merkle_tree
 let insert mt e =
-  let nvalues = insert_values (MT?.values mt) e in
-  let niroots = insert_iroots (MT?.values mt) (MT?.iroots mt) e in
-  MT nvalues niroots
+  let sz = MT?.sz mt in
+  let values = MT?.values mt in
+  let iroots = MT?.iroots mt in
+  MT sz (insert_values sz values e)
+     (insert_iroots iroots 0 (S.length values) e)
 
 /// Getting the Merkle root
 
-val merkle_root_of_hashes: 
-  vs:hash_seq{S.length vs > 0} -> 
-  GTot hash (decreases (S.length vs))
-let rec merkle_root_of_hashes vs =
-  if is_pow2 (S.length vs) then merkle_root_of_pow2 vs
-  else (let lvs, rvs = S.split vs (pow2 (pow2_floor (S.length vs))) in
-       hash_from_hashes (merkle_root_of_pow2 lvs)
-			(merkle_root_of_hashes rvs))
+// val merkle_root_of_hashes: 
+//   vs:hash_seq{S.length vs > 0} -> 
+//   GTot hash (decreases (S.length vs))
+// let rec merkle_root_of_hashes vs =
+//   if is_pow2 (S.length vs) then merkle_root_of_pow2 vs
+//   else (let lvs, rvs = S.split vs (pow2 (pow2_floor (S.length vs))) in
+//        hash_from_hashes (merkle_root_of_pow2 lvs)
+// 			(merkle_root_of_hashes rvs))
 
 val merkle_root_of_iroots: 
   irs:hash_seq{S.length irs > 0} -> 
@@ -351,47 +258,25 @@ let rec merkle_root_of_iroots irs =
   if S.length irs = 1 then S.index irs 0
   else hash_from_hashes (S.head irs) (merkle_root_of_iroots (S.tail irs))
 
-val merkle_root_of_iroots_ok_hashes:
-  vs:hash_seq{S.length vs > 0} ->
-  irs:hash_seq{iroots_of_hashes vs = irs} ->
-  Lemma (ensures (merkle_root_of_iroots irs = merkle_root_of_hashes vs))
-	(decreases (S.length vs))
-let rec merkle_root_of_iroots_ok_hashes vs irs =
-  if is_pow2 (S.length vs) then ()
-  else (let lvs, rvs = S.split vs (pow2 (pow2_floor (S.length vs))) in
-       iroots_of_hashes_head vs irs;
-       iroots_of_hashes_tail vs irs;
-       merkle_root_of_iroots_ok_hashes rvs (S.tail irs))
+// val merkle_root_of_iroots_ok_hashes:
+//   vs:hash_seq{S.length vs > 0} ->
+//   irs:hash_seq{iroots_of_hashes vs = irs} ->
+//   Lemma (ensures (merkle_root_of_iroots irs = merkle_root_of_hashes vs))
+// 	(decreases (S.length vs))
+// let rec merkle_root_of_iroots_ok_hashes vs irs =
+//   if is_pow2 (S.length vs) then ()
+//   else (let lvs, rvs = S.split vs (pow2 (pow2_floor (S.length vs))) in
+//        iroots_of_hashes_head vs irs;
+//        iroots_of_hashes_tail vs irs;
+//        merkle_root_of_iroots_ok_hashes rvs (S.tail irs))
 
-val merkle_root_of_iroots_ok:
-  mt:merkle_tree ->
-  Lemma (requires (S.length (MT?.iroots mt) > 0))
-	(ensures (merkle_root_of_iroots (MT?.iroots mt) = 
-		 merkle_root_of_hashes (MT?.values mt)))
-let merkle_root_of_iroots_ok mt =
-  merkle_root_of_iroots_ok_hashes
-    (MT?.values mt)
-    (MT?.iroots mt)
-
-// assume val hash_init: hash
-// assume val hash_init_idem: 
-//   h:hash -> Lemma (hash_from_hashes h hash_init = h)
-
-// val pad_hashes: hash_seq -> nat -> hash_seq
-// let pad_hashes hs len =
-//   S.append hs (S.create len hash_init)
-
-// val pad_hashes_pow2_ceil:
-//   hs:hash_seq{S.length hs > 0} -> 
-//   GTot (phs:hash_seq{
-//     S.length phs = pow2 (pow2_ceil (S.length hs)) && 
-//     S.slice phs 0 (S.length hs) = hs})
-// let pad_hashes_pow2_ceil hs =
-//   S.append_slices hs (S.create (pow2 (pow2_ceil (S.length hs)) - S.length hs) hash_init);
-//   pad_hashes hs (pow2 (pow2_ceil (S.length hs)) - S.length hs)
-
-// val pad_hashes_pow2_ceil_pow2:
-//   vs:hash_seq{is_pow2 (S.length vs)} ->
-//   Lemma (pad_hashes_pow2_ceil vs = vs)
-// let pad_hashes_pow2_ceil_pow2 vs = ()
+// val merkle_root_of_iroots_ok:
+//   mt:merkle_tree ->
+//   Lemma (requires (S.length (MT?.iroots mt) > 0))
+// 	(ensures (merkle_root_of_iroots (MT?.iroots mt) = 
+// 		 merkle_root_of_hashes (MT?.values mt)))
+// let merkle_root_of_iroots_ok mt =
+//   merkle_root_of_iroots_ok_hashes
+//     (MT?.values mt)
+//     (MT?.iroots mt)
 
